ProvabilityLogic/Logic/GL/Letterless.lean
@@ -1,12 +1,14 @@
 module
 
 public import ProvabilityLogic.Logic.GL.Basic
-public import ProvabilityLogic.Hilbert.Letterless
+public import ProvabilityLogic.Hilbert.GL.Letterless
 
 @[expose]
 public section
 
 variable {α : Type u}
+
+open LogicGL
 
 lemma iff_lift_mem_LogicGL {B : LetterlessFormula} :
     (LetterlessFormula.lift B : Formula α) ∈ LogicGL ↔ B ∈ (LogicGL : Logic Empty) := by
